templates/lockfree/skiplist_v0_search.v
@@ -14,79 +14,156 @@ From iris.bi.lib Require Import fractional.
 Require Export skiplist_v0.
 
 Section skiplist_v0_search.
-  Context {Σ} `{!heapGS Σ, !skG Σ}.
+
+  Context {Σ} `{!heapGS Σ, !dsG Σ, !skG Σ}.
   Notation iProp := (iProp Σ).
 
-  (** Some lemmas *)
-
-(*
-  Parameter ghost_update_keyset : ∀ γ_k dop (k: K) Cn Cn' res K1 C,
-    ⊢   ⌜Ψ dop k Cn Cn' res⌝ 
-      ∗ own γ_k (● prod (KS, C)) 
-      ∗ own γ_k (◯ prod (K1, Cn))
-      ∗ ⌜Cn' ⊆ K1⌝ ∗ ⌜k ∈ K1⌝ ∗ ⌜k ∈ KS⌝ ==∗ 
-        ∃ C', 
-          ⌜Ψ dop k C C' res⌝ 
-        ∗ own γ_k (● prod (KS, C'))
-        ∗ own γ_k (◯ prod (K1, Cn')).
-*)
-
   (** Proofs *)
-    
-  Definition traverse_rec_inv γ_t γ_ght γ_m t_id k s p c : iProp :=
-      past_state γ_t γ_ght γ_m t_id s
+
+  Lemma test γ (N: gset nat) (S: gset proph_id) (F: nat → gset proph_id) :
+    own γ (● S) ∗ ([∗ set] n ∈ N, own γ (◯ (F n))) -∗ 
+      own γ (● S) ∗ ([∗ set] n ∈ N, own γ (◯ (F n))) ∗ ⌜∀ n, n ∈ N → F n ⊆ S⌝.
+  Proof.
+    iInduction N as [| n N] "IH" using set_ind_L.
+    - iIntros "(HS & Hstar)". iFrame. iPureIntro. intros n Hn; set_solver.
+    - iIntros "(HS & Hstar)".
+      rewrite (big_sepS_insert _ N n); last by eauto.
+      iDestruct "Hstar" as "(Hn & Hstar)".
+      iAssert (⌜F n ⊆ S⌝)%I as "%HFn".
+      { admit. }
+      iCombine "HS Hstar" as "H'".
+      iDestruct ("IH" with "H'") as "(HS & star & %IH)".
+      iFrame. iPureIntro. 
+      intros n'. rewrite elem_of_union.
+      intros [Hn | Hn].
+      + assert (n' = n) as -> by set_solver.
+        try done.
+      + apply IH; try done.
+  Admitted.
+      
+  
+  Lemma temporal_interpolation_test1 (M : gmap nat nat) (T: nat) (FP: nat → gset K) :
+      (∀ t, 0 ≤ t < T → FP (M !!! t) ⊆ FP (M !!! (t+1)%nat)) →
+        (∀ t1 t2, 0 ≤ t1 ≤ t2 → t2 < T → FP (M !!! t1) ⊆ FP (M !!! t2)).
+  Proof.
+    intros Hcons. induction t1.
+    - induction t2.
+      + intros; try done.
+      + intros Ht2 Ht2_T.
+        assert (FP (M !!! 0) ⊆ FP (M !!! t2)) as H'.
+        { apply IHt2. lia. lia. }
+        assert (FP (M !!! t2) ⊆ FP (M !!! S t2)) as H''.
+        { assert (t2 + 1 = S t2) as <- by lia.
+          apply Hcons. lia. }
+        clear -H' H''. set_solver.
+    - induction t2.
+      + intros H'. exfalso; lia.
+      + intros Ht1 Ht2_T.
+        assert (FP (M !!! t2) ⊆ FP (M !!! S t2)) as H'.
+        { assert (t2 + 1 = S t2) as <- by lia.
+          apply Hcons. lia. }
+        destruct (decide (S t1 <= t2)).
+        * assert (FP (M !!! S t1) ⊆ FP (M !!! t2)) as H''.
+          { apply IHt2; try lia. }
+          clear -H' H''. set_solver.
+        * assert (t1 = t2) by lia.
+          by subst t1.
+  Qed.
+  
+  Lemma temporal_interpolation_test2 (M : gmap nat nat) 
+    (T t1 t2: nat) (Mark: nat → bool) :
+      (∀ t, 0 ≤ t < T → Mark (M !!! t) = true → Mark (M !!! S t) = true) →
+        Mark (M !!! t1) = false → Mark (M !!! t2) = true → t1 ≤ t2 ≤ T →
+        (∃ t, t1 ≤ t < t2 ∧ Mark (M !!! t) = false ∧ Mark (M !!! S t) = true).
+  Proof.
+    intros Htrans; induction t1; induction t2; 
+    intros Mark1 Mark2 t1_le_t2.
+    - exfalso. rewrite Mark2 in Mark1. inversion Mark1.
+    - destruct (decide (Mark (M !!! t2) = true)). 
+      + assert (0 ≤ t2 ≤ T) as H' by lia.
+        pose proof IHt2 Mark1 e H' as IHt2.
+        destruct IHt2 as [t [Ht [Mark1' Mark2']]].
+        exists t; repeat split; try (done || lia).
+      + exists t2. repeat split; try (done || lia).
+        by rewrite not_true_iff_false in n.
+    - assert (t1 = 0) as -> by lia.
+      assert (0 ≤ 0 < T) as H' by lia.
+      pose proof Htrans 0 H' Mark2 as Htrans.
+      exfalso. rewrite Htrans in Mark1. inversion Mark1.
+    - assert (t1 < t2 ∨ t1 = t2) as Hor by lia.
+      destruct Hor as [Hor | ->].
+      + destruct (decide (Mark (M !!! t2) = true)).
+        * assert (Mark (M !!! t1) = false) as H'.
+          { destruct (decide (Mark (M !!! t1) = false)); try done.
+            rewrite not_false_iff_true in n.
+            assert (0 ≤ t1 < T) as H' by lia.
+            pose proof Htrans t1 H' n as Htrans.
+            rewrite Htrans in Mark1. inversion Mark1. }
+          assert (t1 ≤ S t2 ≤ T) as H'' by lia.
+          pose proof IHt1 H' Mark2 H'' as IHt1.
+          destruct IHt1 as [t [Ht [Mark1' Mark2']]].
+          exists t; repeat split; try (done || lia).
+          assert (t1 < t ∨ t1 = t) as Hor2 by lia.
+          destruct Hor2 as [Hor2 | ->]; try lia.
+          rewrite Mark1 in Mark2'. inversion Mark2'.
+        * rewrite not_true_iff_false in n.
+          exists t2; split; try (done || lia).
+      + rewrite Mark1 in Mark2; inversion Mark2.    
+  Qed.
+  
+  Definition traverse_rec_inv γ_m t0 k s p c : iProp :=
+      past_state γ_m t0 s
     ∗ ⌜p ∈ FP s⌝ ∗ ⌜c ∈ FP s⌝   
     ∗ ⌜¬ mark s p⌝
     ∗ ⌜k ∈ outset K (intf s p) c⌝. 
 
-  Lemma traverse_rec_spec N γ_s γ_t γ_m γ_td γ_ght r t_id (k: K) s p c:
+  Lemma traverse_rec_spec N γ_t γ_s γ_m γ_td γ_ght r γ_sy t_id t0 (k: K) s p c:
     ⌜k ∈ KS⌝ -∗
-      searchstr_inv N γ_s γ_t γ_m γ_td γ_ght r -∗
-       thread_id γ_t γ_ght t_id -∗  
-        traverse_rec_inv γ_t γ_ght γ_m t_id k s p c -∗
-          <<< True >>>
-            traverse_rec r #p #c #k @ (↑(sstrN N))
-          <<< ∃ (p c: Node) (s: State), 
-                past_state γ_t γ_ght γ_m t_id s
-              ∗ ⌜p ∈ FP s⌝ ∗ ⌜c ∈ FP s⌝   
-              ∗ ⌜¬ mark s p⌝
-              ∗ ⌜k ∈ inset K (intf s p) p⌝
-              ∗ ⌜k ∈ outset K (intf s p) c⌝
-              ∗ ⌜¬ mark s c⌝
-              ∗ ⌜k ∈ keyset (intf s c) c⌝, 
-                RET (#p, #c) >>>.
+      css_inv N γ_t γ_s γ_m γ_td γ_ght (skiplist_inv r) -∗
+       thread_vars γ_t γ_ght γ_sy t_id t0 -∗  
+        traverse_rec_inv γ_m t0 k s p c -∗
+          {{{ True }}}
+            traverse_rec r #p #c #k
+          {{{ (p' c': Node) s, RET (#p', #c');
+                past_state γ_m t0 s
+              ∗ ⌜p' ∈ FP s⌝ ∗ ⌜c' ∈ FP s⌝   
+              ∗ ⌜¬ mark s p'⌝
+              ∗ ⌜k ∈ inset K (intf s p') p'⌝
+              ∗ ⌜k ∈ outset K (intf s p') c'⌝
+              ∗ ⌜¬ mark s c'⌝
+              ∗ ⌜k ∈ keyset (intf s c')⌝ }}}.
   Proof.
-    iIntros "%k_in_KS #HInv #Htid". 
+    iIntros "%k_in_KS #HInv #Thd". 
     iLöb as "IH" forall (s p c). 
-    iIntros "#Tr_inv" (Φ) "AU".
-    wp_lam. wp_pures. awp_apply (findNext_spec).
-    iInv "HInv" as (s0 M0 T0) "(>Half & >Res & >Hist & Help)".
+    iIntros "#Tr_inv" (Φ) "!# _ Hpost".
+    wp_lam. wp_pures. awp_apply (findNext_spec); try done.
+    iInv "HInv" as (M0 T0 s0) "(>CSS & >%Habs0 & >Hist & Help & >Templ)".
+    { admit. }
+    iDestruct "Templ" as "(PT & %Trans_M & %Trans_s & Res)". 
     iAssert (⌜c ∈ FP s0⌝)%I as %FP_c.
     { admit. }
-    iDestruct "Res" as "(Per_tick & Resources)".
-    iEval (unfold resources) in "Resources". 
     rewrite (big_sepS_delete _ (FP s0) c); last by eauto.
-    iDestruct "Resources" as "(NodeFull_c & Resources_rest)".
+    iDestruct "Res" as "(NodeFull_c & Res_rest)".
     iDestruct "NodeFull_c" as (mc Ic pcc) "(Node & Node_rest)".
     iAaccIntro with "Node".
-    { iIntros "Node". iModIntro. iFrame "AU". 
-      iNext; iExists s0, M0, T0.
-      iFrame. unfold resources. 
+    { iIntros "Node". iModIntro. iFrame "Hpost". 
+      iNext; iExists M0, T0, s0.
+      iFrame "∗#%". 
       rewrite (big_sepS_delete _ (FP s0) c); last by eauto. 
-      iFrame "Resources_rest".
+      iFrame "Res_rest".
       iExists mc, Ic, pcc. iFrame. }
     iIntros (succ n) "(Node & Hif)".
     destruct mc; destruct succ.
-    - iModIntro. iSplitR "AU".
+    - iModIntro. iSplitR "Hpost".
       { admit. }
       wp_pures. awp_apply (try_constraint_trav_spec _ k).
-      iInv "HInv" as (s1 M1 T1) "(>Half & >Res & >Hist & Help)".
+      iInv "HInv" as (M1 T1 s1) "(>CSS & >%Habs1 & >Hist & Help & >Templ)".
+      { admit. }
       iAssert (⌜p ∈ FP s1⌝)%I as %FP_p.
       { admit. }
-      iDestruct "Res" as "(Per_tick & Resources)".
-      iEval (unfold resources) in "Resources". 
+      iDestruct "Templ" as "(PT & %Trans_M1 & %Trans_s1 & Res)".
       rewrite (big_sepS_delete _ (FP s1) p); last by eauto.
-      iDestruct "Resources" as "(NodeFull_p & Resources_rest)".
+      iDestruct "Res" as "(NodeFull_p & Res_rest)".
       iDestruct "NodeFull_p" as (mp Ip pcp) "(Node & Node_rest)".
       iAaccIntro with "Node".
       { iIntros "Node". admit. }
@@ -94,58 +171,60 @@ Section skiplist_v0_search.
       destruct succ.
       + iDestruct "Hif" as %((mp_false & k_in_Ip_c) & k_in_Ip'_n).
         admit.
-      + iModIntro. iSplitR "AU".
+      + iModIntro. iSplitR "Hpost".
         { admit. } 
         wp_pures.
         admit.
-    - iModIntro. iSplitR "AU".
+    - iModIntro. iSplitR "Hpost".
       { admit. }
       wp_pures. iExFalso. admit.
-    - iModIntro. iSplitR "AU".
+    - iModIntro. iSplitR "Hpost".
       { admit. } 
       wp_pures. admit.
   Admitted.
 
-
-  Lemma traverse_spec N γ_s γ_t γ_m γ_td γ_ght r t_id (k: K) :
+  Lemma traverse_spec N γ_t γ_s γ_m γ_td γ_ght r γ_sy t_id t0 (k: K) :
     ⌜k ∈ KS⌝ -∗
-      searchstr_inv N γ_s γ_t γ_m γ_td γ_ght r -∗
-       thread_id γ_t γ_ght t_id -∗ 
-        <<< True >>>
-           traverse r #k @ (↑(sstrN N))
-        <<< ∃ (p c: Node) (s: State), 
-              past_state γ_t γ_ght γ_m t_id s
+      css_inv N γ_t γ_s γ_m γ_td γ_ght (skiplist_inv r) -∗
+       thread_vars γ_t γ_ght γ_sy t_id t0 -∗  
+        {{{ True }}}
+           traverse r #k
+        {{{ (p c: Node) s, RET (#p, #c); 
+              past_state γ_m t0 s
             ∗ ⌜p ∈ FP s⌝ ∗ ⌜c ∈ FP s⌝   
             ∗ ⌜¬ mark s p⌝
             ∗ ⌜k ∈ inset K (intf s p) p⌝
             ∗ ⌜k ∈ outset K (intf s p) c⌝
             ∗ ⌜¬ mark s c⌝
-            ∗ ⌜k ∈ keyset (intf s c) c⌝, 
-              RET (#p, #c) >>>.
+            ∗ ⌜k ∈ keyset (intf s c)⌝ }}}.
   Proof.
-    iIntros "%k_in_KS #HInv #Htid" (Φ) "AU".
-    wp_lam. awp_apply (findNext_spec).
-    iInv "HInv" as (s0 M0 T0) "(>Half & >Res & >Hist & Help)".
+    iIntros "%k_in_KS #HInv #Thd". iIntros (Φ) "!# _ Hpost".
+    wp_lam. awp_apply (findNext_spec); try done.
+    iInv "HInv" as (M0 T0 s0) "(>CSS & >%Habs0 & >Hist & Help & >Templ)".
+    { admit. }
+    iDestruct "Templ" as "(PT & %Trans_M & %Trans_s & Res)". 
     iAssert (⌜r ∈ FP s0⌝)%I as %FP_r0.
     { admit. }
-    iDestruct "Res" as "(Per_tick & Resources)".
-    iEval (unfold resources) in "Resources". 
     rewrite (big_sepS_delete _ (FP s0) r); last by eauto.
-    iDestruct "Resources" as "(NodeFull_r & Resources_rest)".
+    iDestruct "Res" as "(NodeFull_r & Res_rest)".
     iDestruct "NodeFull_r" as (mr Ir pcr) "(Node & Node_rest)".
     iAaccIntro with "Node".
-    { iIntros "Node". iModIntro. iFrame "AU". 
-      iNext; iExists s0, M0, T0.
-      iFrame. unfold resources. 
+    { iIntros "Node". iModIntro. iFrame "Hpost". 
+      iNext; iExists M0, T0, s0.
+      iFrame "∗#%". 
       rewrite (big_sepS_delete _ (FP s0) r); last by eauto. 
-      iFrame "Resources_rest".
+      iFrame "Res_rest".
       iExists mr, Ir, pcr. iFrame. }
     iIntros (succ n) "(Node & Hif)".
     destruct succ; last first.
     - iAssert (⌜k ∉ KS⌝)%I as %k_notin_KS.
-      { iAssert (⌜T0 ∈ dom (gset nat) M0⌝)%I as %t_in_M0.
+      { iAssert (⌜T0 ∈ dom M0⌝)%I as %t_in_M0.
         { admit. }
-        iDestruct "Per_tick" as "(HI & HKS & Ins_r & Out_r 
+        rewrite (big_sepS_delete _ (dom M0) T0); last by eauto.
+        iDestruct "PT" as "(PT_T0 & PT_rest)".
+        iAssert (per_tick_inv r (s0))%I with "[PT_T0]" as "PT_T0".
+        { admit. }
+        iDestruct "PT_T0" as "(HI & HKS & Ins_r & Out_r 
           & Mark_r & Hbig_star)".
         iDestruct "Hif" as %Hif.
         iDestruct "Out_r" as %Out_r.
@@ -154,21 +233,18 @@ Section skiplist_v0_search.
         by rewrite Out_r in Hif. }
       iClear "∗#". clear -k_in_KS k_notin_KS. exfalso; try done.
     - iModIntro.
-      iDestruct "Htid" as (t0 γ_sy)"Htid".
-      iAssert (own γ_m (◯ {[T0 := to_agree s0]}))%I as "#HT0".
-      { admit. }
-      iAssert (⌜t0 ≤ T0⌝)%I as %t0_le_T0.
-      { admit. }
-      iAssert (past_state γ_t γ_ght γ_m t_id s0)%I as "#Hpast".
-      { iExists t0, γ_sy, T0. iFrame "#%". }
-      iAssert (⌜r ∈ FP s0⌝)%I as %FP_r.
+      iAssert (past_state γ_m t0 s0)%I as "#Hist_s0".
       { admit. }
       iAssert (⌜n ∈ FP s0⌝)%I as %FP_n.
       { admit. }
-      iAssert (⌜T0 ∈ dom (gset nat) M0⌝)%I as %T0_in_M0.
+      iAssert (⌜T0 ∈ dom M0⌝)%I as %T0_in_M0.
       { admit. }
-      iDestruct "Per_tick" as "(HI & HKS & %Ins_r & %Out_r 
-          & %Mark_r & Hbig_star)".    
+      rewrite (big_sepS_delete _ (dom M0) T0); last by eauto.
+      iDestruct "PT" as "(PT_T0 & PT_rest)".
+      iAssert (per_tick_inv r (s0))%I with "[PT_T0]" as "PT_T0".
+      { admit. }
+      iDestruct "PT_T0" as "(HI & HKS & %Ins_r & %Out_r 
+          & %Mark_r & Hbig_star)".
       iAssert (⌜k ∈ inset K (intf s0 r) r⌝)%I as %k_in_Insr.
       { iPureIntro. by rewrite Ins_r. }
       iDestruct "Hif" as %k_in_Outr.
@@ -177,82 +253,93 @@ Section skiplist_v0_search.
       iAssert (⌜n ∈ FP s0 ∖ {[r]}⌝)%I as "%".
       { clear -FP_n n_neq_r. iPureIntro; set_solver. } 
       rewrite (big_sepS_delete _ (FP s0 ∖ {[r]}) n); last by eauto.
-      iDestruct "Resources_rest" as "(NodeFull_n & Resources_rest)".
+      iDestruct "Res_rest" as "(NodeFull_n & Res_rest)".
       iDestruct "NodeFull_n" as (mn In pcn) "(Node_n & Node_n_rest)".
       iAssert (⌜Ir = intf s0 r⌝)%I as %HIr.
       { by iDestruct "Node_rest" as "(_&%&_)". }
       rewrite HIr in k_in_Outr.
       iAssert (⌜k ∈ inset K (intf s0 n) n⌝)%I as %k_in_Insn.
       { admit. }
-      iAssert (traverse_rec_inv γ_t γ_ght γ_m t_id k s0 r n)%I as "#Tr_inv".
+      iAssert (traverse_rec_inv γ_m t0 k s0 r n)%I as "#Tr_inv".
       { iFrame "#%". }
-      iSplitR "AU". 
-      { iNext. iExists s0, M0, T0.
-        iFrame "Half Hist Help". iFrame.
-        iSplitR. iPureIntro; repeat split; try done.
-        unfold resources. 
-        rewrite (big_sepS_delete _ (FP s0) r); last by eauto.
+      iSplitR "Hpost". 
+      { iNext. iExists M0, T0, s0.
+        iFrame "∗#%".
+        rewrite (big_sepS_delete _ (dom M0) T0); last by eauto.
+        iFrame. iSplitL "HI HKS Hbig_star".
+        { admit. }
+        rewrite (big_sepS_delete (nodeFull s0) (FP s0) r); last by eauto.
         rewrite (big_sepS_delete _ (FP s0 ∖ {[r]}) n); last by eauto.
-        iFrame "Resources_rest". iSplitL "Node Node_rest". 
+        iFrame. iSplitL "Node Node_rest". 
         iExists mr, Ir, pcr. iFrame.
         iExists mn, In, pcn. iFrame. }   
-      wp_pures. awp_apply traverse_rec_spec; try done.
-      { by iExists t0, γ_sy. }
-      iAaccIntro with ""; try done.
-      { iIntros "_". iModIntro. iFrame. }
-      iIntros (p c s) "Hpost".
-      iMod "AU" as "[_ [_ Hcomm]]".
-      iSpecialize ("Hcomm" $! p c s).
-      iMod ("Hcomm" with "Hpost") as "HΦ".
-      by iModIntro.  
+      wp_pures. wp_apply traverse_rec_spec; try done.
   Admitted.
 
   
-  Lemma search_spec N γ_s γ_t γ_m γ_td γ_ght r t_id (k: K) :
-    ⌜k ∈ KS⌝ -∗
-      searchstr_inv N γ_s γ_t γ_m γ_td γ_ght r -∗
-        thread_id γ_t γ_ght t_id -∗ 
-          <<< True >>>
-            search r #k @ ⊤ ∖ (↑(sstrN N))
-          <<< ∃ (res: bool) (s: State), 
-                past_state γ_t γ_ght γ_m t_id s 
-              ∗ ⌜seq_spec k (gcont s) res⌝, 
-                RET #res >>>.
+  Parameter ghost_update_keyset : ∀ γ_k dop (k: K) Cn Cn' res K1 C,
+    ⊢   ⌜seq_spec dop Cn Cn' res k⌝ 
+      ∗ own γ_k (● prod (KS, C)) 
+      ∗ own γ_k (◯ prod (K1, Cn))
+      ∗ ⌜Cn' ⊆ K1⌝ ∗ ⌜k ∈ K1⌝ ∗ ⌜k ∈ KS⌝ ==∗ 
+        ∃ C', 
+          ⌜seq_spec dop C C' res k⌝ 
+        ∗ own γ_k (● prod (KS, C'))
+        ∗ own γ_k (◯ prod (K1, Cn')).
+(*
+  Parameter ghost_update_keyset_search : ∀ γ_k (k: K) Cn res K1 C,
+    ⊢   ⌜seq_spec searchOp Cn Cn res k⌝ 
+      ∗ own γ_k (● prod (KS, C)) 
+      ∗ own γ_k (◯ prod (K1, Cn))
+      ∗ ⌜Cn' ⊆ K1⌝ ∗ ⌜k ∈ K1⌝ ∗ ⌜k ∈ KS⌝ ==∗  
+          ⌜seq_spec searchOp C C' res k⌝ 
+        ∗ own γ_k (● prod (KS, C'))
+        ∗ own γ_k (◯ prod (K1, Cn')).
+*)
+
+  
+  Lemma searchOp_spec N γ_s γ_t γ_m γ_td γ_ght r (k: K) γ_sy t_id t0:
+        ⌜k ∈ KS⌝ -∗
+          css_inv N γ_t γ_s γ_m γ_td γ_ght (skiplist_inv r) -∗
+            □ update_helping_protocol N γ_t γ_s γ_td γ_ght -∗
+              thread_vars γ_t γ_ght γ_sy t_id t0 -∗
+                {{{ True }}} 
+                     search r #k
+                {{{ res, RET #res; past_lin_witness γ_m searchOp k res t0  }}}.
   Proof.
-    iIntros "% #HInv #Htid" (Φ) "AU".
-    rename H into k_in_KS.
+    iIntros "%k_in_KS #HInv #HUpd #Thd". iIntros (Φ) "!# _ Hpost".
     wp_lam. wp_pures.
-    awp_apply traverse_spec; try done.
-    iAaccIntro with ""; try done.
-    { eauto with iFrame. }
+    wp_apply traverse_spec; try done.
     iIntros (p c s) "(#Hpast & %)".
-    destruct H as [FP_p [FP_c [Unmarkedp [k_in_pins 
-      [k_in_pouts [Unmarkedc k_in_cks]]]]]].
-    iModIntro. wp_pures.
-    awp_apply (inContents_spec).
-    iInv "HInv" as (s0 M0 T0) "(>Half & >Res & >Hist & Help)".
+    destruct H as [FP_p [FP_c [Unmarked_p [k_in_ins_p 
+      [k_in_outs_p [Unmarked_c k_in_ks_c]]]]]].
+    wp_pures.
+    awp_apply (inContents_spec); try done.
+    iInv "HInv" as (M0 T0 s0) "(>CSS & >%Habs0 & >Hist & Help & >Templ)".
+    { admit. }
+    iDestruct "Templ" as "(PT & %Trans_M1 & %Trans_s1 & Res)". 
     iAssert (⌜c ∈ FP s0⌝)%I as %FP_p0.
     { (* interpolation *) admit. }
-    iDestruct "Res" as "(Per_tick & Resources)".
-    iEval (unfold resources) in "Resources". 
     rewrite (big_sepS_delete _ (FP s0) c); last by eauto.
-    iDestruct "Resources" as "(NodeFull_c & Resources_rest)".
+    iDestruct "Res" as "(NodeFull_c & Res_rest)".
     iDestruct "NodeFull_c" as (mc Ic pcc) "(Node & Node_rest)".
     iAaccIntro with "Node".
-    { iIntros "Node". iModIntro. iFrame "AU". 
-      iNext; iExists s0, M0, T0.
-      iFrame. unfold resources. 
+    { iIntros "Node". iModIntro. iFrame "Hpost". 
+      iNext; iExists M0, T0, s0.
+      iFrame "∗%#". 
       rewrite (big_sepS_delete _ (FP s0) c); last by eauto. 
-      iFrame "Resources_rest".
+      iFrame "Res_rest".
       iExists mc, Ic, pcc. iFrame. }
     iIntros (res) "(Node & Hres)". iDestruct "Hres" as %Hres.
-    iAssert (past_state γ_t γ_ght γ_m t_id s)%I as "#Hpast2". { done. }
-    iDestruct "Hpast2" as (t0 γ_sy t)"(Hth_vars & t_s & %)".
-    iAssert (⌜t ∈ dom (gset nat) M0⌝)%I as %t_in_M0.
+    iSpecialize ("Hpost" $! res).
+
+    iAssert (past_state γ_m t0 s)%I as "#Hpast2". { done. }
+    iDestruct "Hpast2" as (t)"(%t0_le_t & #Hist_s)".
+    iAssert (⌜t ∈ dom M0⌝)%I as %t_in_M0.
     { admit. }
-(*    
-    rewrite (big_sepS_delete _ (dom (gset nat) M0) t); last by eauto.
-    iDestruct "Per_tick" as "(Tick_t & Per_tick_rest)".
+
+    rewrite (big_sepS_delete _ (dom M0) t); last by eauto.
+    iDestruct "PT" as "(Tick_t & PT_rest)".
     iAssert (⌜M0 !!! t = s⌝)%I as %M0_t_s.
     { admit. } iEval (rewrite M0_t_s) in "Tick_t". 
     iDestruct "Tick_t" as "(HI & HKS & Ins_r & Out_r & Mark_r & Hbig_star)".
@@ -261,40 +348,54 @@ Section skiplist_v0_search.
     iDestruct "Node_local" as "(HIc & Hksc & Hpurec)".
     iAssert (⌜pcc = PC s c⌝)%I as %->.
     { (* interpolation *) admit. }
-    iAssert (⌜Ψ searchOp k (C s c) (C s c) res⌝)%I as %HΨ_c.
-    { iPureIntro. unfold Ψ. split; try done. destruct res; 
-      unfold C; destruct (decide (mark s c)); try done.
+    iAssert (⌜seq_spec searchOp (Cont s c) (Cont s c) res k⌝)%I as %Seq_spec_c.
+    { iPureIntro. unfold seq_spec. split; try done. destruct res; 
+      unfold Cont; destruct (decide (mark s c)); try done.
       - by apply Hres.
       - intros ?. by apply Hres. }
-    iAssert (⌜C s c ⊆ keyset (intf s c) c⌝)%I as %cc_sub_ksc.
+    iAssert (⌜Cont s c ⊆ keyset (intf s c)⌝)%I as %cc_sub_ksc.
     { by iDestruct "Hpurec" as "(_ & % & _)". }
-    iMod (ghost_update_keyset (γ_ks s) searchOp k (C s c) (C s c) res 
-      (keyset (intf s c) c) (gcont s)
-      with "[$HKS $Hksc]") as (C') "(% & HKS & Hksc)".
+    iAssert (⌜seq_spec searchOp (abs s) (abs s) res k⌝)%I as %Seq_spec.
+    { iPureIntro. unfold seq_spec. split; try done. destruct res.
+      - assert (k ∈ Cont s c) as H'.
+        { unfold Cont. rewrite decide_False; try done.
+          by apply Hres. }
+        assert (Cont s c ⊆ abs s) as H''.
+        { admit. }
+        clear -H' H''; set_solver.
+      - (* Need this property from all snapshots *)
+        assert (∀ s n k, k ∈ keyset (intf s n) → (k ∈ (Cont s n) ↔ k ∈ abs s)).
+        { admit. }
+        admit. }
+(*        
+    iMod (ghost_update_keyset (γ_ks s) searchOp k (Cont s c) (Cont s c) res 
+      (keyset (intf s c)) (abs s)
+      with "[$HKS $Hksc]") as (C') "(%Seq_spec & HKS & Hksc)".
     { iPureIntro; repeat (split; try done). }
-    rename H0 into HΨ.
-    iAssert (⌜C' = gcont s⌝)%I as %->.
-    { by destruct HΨ as [? _]. }
-    iAssert (⌜search_seq_spec k (gcont s) res⌝)%I as %HPost.
-    { by iPureIntro. }
-    iMod "AU" as "[_ [_ Hcomm]]". admit.
-    iSpecialize ("Hcomm" $! res s).
-    iMod ("Hcomm" with "[$Hpast]") as "HΦ".
-    { by iPureIntro. }
-    
-    iModIntro. iFrame "HΦ". 
-    { iNext. iExists T0, s0, M0, M0'.
-      iFrame "Half Hist Help". iFrame "Trans_inv".
-      iSplitR "Node Node_rest Resources_rest".
-      rewrite (big_sepS_delete _ (dom (gset nat) M0) t); last by eauto.
-      iFrame "Per_tick_rest". iEval (rewrite M0_t_s). iFrame "HI HKS".
+    iAssert (⌜C' = abs s⌝)%I as %->.
+    { by destruct Seq_spec as [? _]. }
+*)    
+    iAssert (past_lin_witness γ_m searchOp k res t0) as "Witn".
+    { unfold past_lin_witness, updater_thread. iExists s.
+      iFrame "#". by iPureIntro. }
+
+    iModIntro. iSplitR "Hpost"; last first.
+    { iApply "Hpost"; try done. } 
+    { iNext. iExists M0, T0, s0.
+      iFrame "CSS Hist Help %".
+      iSplitR "Node Node_rest Res_rest".
+      rewrite (big_sepS_delete _ (dom M0) t); last by eauto.
+      iFrame "PT_rest". iEval (rewrite M0_t_s). iFrame "HI HKS".
       rewrite (big_sepS_delete _ (FP s) c); last by eauto.
       iFrame"Hbig_star_rest". iFrame.
-      unfold resources. 
       rewrite (big_sepS_delete _ (FP s0) c); last by eauto.
-      iFrame "Resources_rest". iExists mc, Ic, (PC s c). iFrame. }
-*)      
+      iFrame "Res_rest". iExists mc, Ic, (PC s c). iFrame. }
   Admitted.      
+    
+                  
+
+
+    
           
 End skiplist_v0_search.            
       
