templates/lockfree/skiplist_v0_insert.v
@@ -1,0 +1,57 @@
+From iris.proofmode Require Import tactics.
+From iris.heap_lang Require Import proofmode par.
+From iris.heap_lang.lib Require Import nondet_bool.
+From iris.bi.lib Require Import fractional.
+Set Default Proof Using "All".
+From iris.bi.lib Require Import fractional.
+Require Export skiplist_v0 skiplist_v0_search.
+
+Section skiplist_v0_search.
+
+  Context {Σ} `{!heapGS Σ, !dsG Σ, !skG Σ}.
+  Notation iProp := (iProp Σ).
+  
+  (* Proofs *)
+
+  Lemma insertOp_spec N γ_s γ_t γ_m γ_td γ_ght r (k: K) γ_sy t_id t0:
+        ⌜k ∈ KS⌝ -∗
+          css_inv N γ_t γ_s γ_m γ_td γ_ght (skiplist_inv r) -∗
+            □ update_helping_protocol N γ_t γ_s γ_td γ_ght -∗
+              thread_vars γ_t γ_ght γ_sy t_id t0 -∗
+                {{{ True }}} 
+                     insert r #k
+                {{{ res, RET #res; past_lin_witness γ_m insertOp k res t0  }}}.
+  Proof.
+    iIntros "%k_in_KS #HInv #Thd". iLöb as "IH".
+    iIntros "#Tr_inv" (Φ) "!# _ Hpost".
+    wp_lam. wp_apply traverse_spec; try done.
+    iIntros (p c s) "(#Hpast & %)".
+    destruct H as [FP_p [FP_c [Unmarked_p [k_in_ins_p 
+      [k_in_outs_p [Unmarked_c k_in_ks_c]]]]]].
+    wp_pures.
+    awp_apply (inContents_spec); try done.
+    iInv "HInv" as (M0 T0 s0) "(>CSS & >%Habs0 & >Hist & Help & >Templ)".
+    { admit. }
+    iDestruct "Templ" as "(PT & %Trans_M1 & %Trans_s1 & Res)". 
+    iAssert (⌜c ∈ FP s0⌝)%I as %FP_p0.
+    { (* interpolation *) admit. }
+    rewrite (big_sepS_delete _ (FP s0) c); last by eauto.
+    iDestruct "Res" as "(NodeFull_c & Res_rest)".
+    iDestruct "NodeFull_c" as (mc Ic pcc) "(Node & Node_rest)".
+    iAaccIntro with "Node".
+    { iIntros "Node". iModIntro. iFrame "Hpost". 
+      iNext; iExists M0, T0, s0.
+      iFrame "∗%#". 
+      rewrite (big_sepS_delete _ (FP s0) c); last by eauto. 
+      iFrame "Res_rest".
+      iExists mc, Ic, pcc. iFrame. }
+    iIntros (res) "(Node & Hres)". iDestruct "Hres" as %Hres.
+    iSpecialize ("Hpost" $! res).
+    destruct res.
+    
+    
+    
+    
+  Admitted.    
+    
+  
